src/program_proof/memkv/memkv_shard_make_proof.v
@@ -10,8 +10,8 @@ Context `{!heapGS Σ, erpcG Σ ShardReplyC, urpcregG Σ, kvMapG Σ}.
 
 Lemma wp_MakeKVShardServer (b : bool) γ :
   {{{
-       "#His_srv" ∷ is_RPCServer γ.(rpc_gn) ∗
-       "HRPCserver_own" ∷ RPCServer_own_ghost γ.(rpc_gn) ∅ ∅ ∗
+       "#His_srv" ∷ is_eRPCServer γ.(rpc_gn) ∗
+       "HRPCserver_own" ∷ eRPCServer_own_ghost γ.(rpc_gn) ∅ ∅ ∗
        "HghostShards" ∷ (if b then [∗ set] sid ∈ rangeSet 0 uNSHARD, own_shard γ.(kv_gn) sid ∅ else True) ∗
        "Hcids" ∷ [∗ set] cid ∈ (fin_to_set u64), is_eRPCClient_ghost γ.(rpc_gn) cid 1
   }}}
